Complete asgn08.

sf/Assignment08_05.v
@@ -7,7 +7,13 @@ Require Export Assignment08_04.
     same as pushing the value of the expression on the stack. *)
 
 Fixpoint s_compile (e : aexp) : list sinstr :=
-  FILL_IN_HERE.
+  match e with
+    | ANum n => [SPush n]
+    | AId x => [SLoad x]
+    | APlus e1 e2 => (s_compile e1) ++ (s_compile e2) ++ [SPlus]
+    | AMinus e1 e2 => (s_compile e1) ++ (s_compile e2) ++ [SMinus]
+    | AMult e1 e2 => (s_compile e1) ++ (s_compile e2) ++ [SMult]
+  end.
 
 (** After you've defined [s_compile], prove the following to test
     that it works. *)
@@ -16,7 +22,7 @@ Example s_compile1 :
     s_compile (AMinus (AId X) (AMult (ANum 2) (AId Y)))
   = [SLoad X; SPush 2; SLoad Y; SMult; SMinus].
 Proof.
-  exact FILL_IN_HERE.
+  reflexivity.
 Qed.
 
 (** **** Exercise: 3 stars, advanced (stack_compiler_correct)  *)
@@ -33,10 +39,25 @@ Qed.
     general lemma to get a usable induction hypothesis; the main
     theorem will then be a simple corollary of this lemma. *)
 
+Lemma s_compile_correct_helper:
+  forall (st : state) (e : aexp) (ln : list nat) (more : list sinstr),
+    s_execute st ln ((s_compile e) ++ more) =
+    s_execute st ([ aeval st e] ++ ln) more.
+  intros st e.
+  induction e; intros; try (simpl;reflexivity);
+  try (simpl; rewrite <- app_assoc; rewrite -> IHe1; simpl;
+       rewrite <- app_assoc; rewrite -> IHe2; simpl; reflexivity).
+Qed.
+
 Theorem s_compile_correct : forall (st : state) (e : aexp),
   s_execute st [] (s_compile e) = [ aeval st e ].
 Proof.
-  exact FILL_IN_HERE.
+  intros.
+  assert (Hsp: s_execute st [] ((s_compile e) ++ []) =
+               s_execute st ([ aeval st e] ++ []) []).
+  { apply s_compile_correct_helper. }
+  simpl in Hsp. rewrite -> app_nil_r in Hsp.
+  apply Hsp.
 Qed.
 
 (*-- Check --*)
