sf/Assignment08_01.v
@@ -7,7 +7,14 @@ Example ceval_example2:
     (X ::= ANum 0;; Y ::= ANum 1;; Z ::= ANum 2) / empty_state ||
     (update (update (update empty_state X 0) Y 1) Z 2).
 Proof.
-  exact FILL_IN_HERE.
+  eapply E_Seq.
+  {
+    constructor.
+    simpl.
+    reflexivity.
+  }
+  eapply E_Seq;
+   constructor; simpl; reflexivity.
 Qed.
 
 (*-- Check --*)
