sf/Assignment08_02.v
@@ -9,14 +9,67 @@ Require Export Assignment08_01.
    (this latter part is trickier than you might expect). *)
 
 Definition pup_to_n : com :=
-  FILL_IN_HERE.
+  Y ::= (ANum 0);;
+  WHILE (BLe (ANum 1) (AId X)) DO
+    Y ::= APlus (AId Y) (AId X);;
+    X ::= AMinus (AId X) (ANum 1)
+  END
+  .
+    
 
 Example pup_to_2_ceval :
   pup_to_n / (update empty_state X 2) ||
     update (update (update (update (update (update empty_state
       X 2) Y 0) Y 2) X 1) Y 3) X 0.
 Proof.
-  exact FILL_IN_HERE.
+  eapply E_Seq.
+  {
+    constructor.
+    simpl. reflexivity.
+  }
+  eapply E_WhileLoop.
+  {
+    simpl.
+    reflexivity.
+  }
+  {
+    eapply E_Seq.
+    {
+      constructor.
+      simpl.
+      unfold update.
+      destruct (eq_id_dec Y X).
+      - inversion e.
+      - simpl. 
+        reflexivity.
+    }
+    constructor.
+    simpl.
+    reflexivity.
+  }
+  eapply E_WhileLoop.
+  {
+    simpl.
+    reflexivity.
+  }
+  {
+    eapply E_Seq.
+    {
+      constructor.
+      simpl.
+      unfold update.
+      destruct (eq_id_dec Y X).
+      - inversion e.
+      - simpl. 
+        reflexivity.
+    }
+    constructor.
+    simpl.
+    reflexivity.
+  }
+  eapply E_WhileEnd.
+  simpl.
+  reflexivity.
 Qed.
 
 (*-- Check --*)
