sf/Assignment08_04.v
@@ -13,7 +13,36 @@ Theorem no_whiles_terminate: forall c st
     (NOWHL: no_whiles c = true),
   exists st', c / st || st'.
 Proof.
-  exact FILL_IN_HERE.
+  intros c.
+  induction c; intros.
+  - exists st. constructor.
+  - exists (update st i (aeval st a)).
+    constructor. reflexivity.
+  - simpl in NOWHL.
+    symmetry in NOWHL.
+    apply andb_true_eq in NOWHL.
+    destruct NOWHL as [NW1 NW2].
+    symmetry in NW1, NW2.
+    apply (IHc1 st) in NW1.
+    destruct NW1 as [st1 CEV1].
+    apply (IHc2 st1) in NW2.
+    destruct NW2 as [st2 CEV2].
+    eexists. econstructor.
+    apply CEV1.
+    apply CEV2.
+  - simpl in NOWHL.
+    symmetry in NOWHL.
+    apply andb_true_eq in NOWHL.
+    destruct NOWHL as [NW1 NW2].
+    symmetry in NW1, NW2.
+    apply (IHc1 st) in NW1.
+    destruct NW1 as [st1 CEV1].
+    apply (IHc2 st) in NW2.
+    destruct NW2 as [st2 CEV2].
+    destruct (beval st b) eqn:EVb;
+      eexists; [apply E_IfTrue | apply E_IfFalse]; eauto.
+  - simpl in NOWHL.
+    inversion NOWHL.
 Qed.
 
 (*-- Check --*)
