sf/Assignment08_08.v
@@ -11,7 +11,18 @@ Theorem swap_if_branches: forall b e1 e2,
     (IFB b THEN e1 ELSE e2 FI)
     (IFB BNot b THEN e2 ELSE e1 FI).
 Proof.
-  exact FILL_IN_HERE.
+  intros.
+  split; intros Has.
+  - destruct (beval st b) eqn:HEVb; inversion Has; subst;
+    try (rewrite -> HEVb in H4; inversion H4).
+    + apply E_IfFalse; auto.
+      simpl. rewrite -> HEVb. reflexivity.
+    + apply E_IfTrue; auto.
+      simpl. rewrite -> HEVb. reflexivity.
+  - destruct (beval st b) eqn:HEVb; inversion Has; subst;
+    try (simpl in H4; rewrite -> HEVb in H4; inversion H4).
+    + apply E_IfTrue; auto.
+    + apply E_IfFalse; auto.
 Qed.
 
 (*-- Check --*)
