sf/Assignment08_11.v
@@ -7,7 +7,29 @@ Theorem assign_aequiv : forall X e,
   aequiv (AId X) e -> 
   cequiv SKIP (X ::= e).
 Proof.
-  exact FILL_IN_HERE.
+  intros.
+  split; intros Has.
+  - replace st' with (update st X (aeval st e)).
+    + constructor. reflexivity.
+    + unfold aequiv in H.
+      inversion Has. subst.
+      apply functional_extensionality.
+      intros Y. unfold update.
+      destruct (eq_id_dec X Y).
+      * rewrite <- H. subst. simpl. reflexivity.
+      * reflexivity.
+  - inversion Has. subst.
+    assert (STEQ: st = update st X (aeval st e)).
+    {
+      apply functional_extensionality.
+      intros Y.
+      unfold update.
+      destruct (eq_id_dec X Y).
+      - rewrite <- H. subst. simpl. reflexivity.
+      - reflexivity.
+    }
+    rewrite <- STEQ.
+    constructor.
 Qed.
 
 (*-- Check --*)
