sf/Assignment08_13.v
@@ -7,7 +7,24 @@ Theorem CIf_congruence : forall b b' c1 c1' c2 c2',
   bequiv b b' -> cequiv c1 c1' -> cequiv c2 c2' ->
   cequiv (IFB b THEN c1 ELSE c2 FI) (IFB b' THEN c1' ELSE c2' FI).
 Proof.
-  exact FILL_IN_HERE.
+  intros.
+  split.
+  - intros HEVc.
+    inversion HEVc; subst.
+    + apply E_IfTrue.
+      * rewrite <- H; auto.
+      * apply H0; auto.
+    + apply E_IfFalse.
+      * rewrite <- H ; auto.
+      * apply H1; auto.
+  - intros HEVc.
+    inversion HEVc; subst.
+    + apply E_IfTrue.
+      * rewrite -> H; auto.
+      * apply H0; auto.
+    + apply E_IfFalse.
+      * rewrite -> H ; auto.
+      * apply H1; auto.
 Qed.
 
 (*-- Check --*)
