sf/Assignment08_16.v
@@ -5,7 +5,24 @@ Require Export Assignment08_15.
 Lemma optimize_0plus_aexp_sound:
   atrans_sound optimize_0plus_aexp.
 Proof.
-  exact FILL_IN_HERE.
+  unfold atrans_sound. intros. unfold aequiv. intros.
+  induction a.
+  - simpl. reflexivity.
+  - simpl. reflexivity.
+  - simpl.
+    remember (optimize_0plus_aexp a1) as a1' eqn:Ha1'.
+    remember (optimize_0plus_aexp a2) as a2' eqn:Ha2'.
+    destruct a1; destruct a2; try (destruct n);
+    try (rewrite -> IHa1; rewrite -> IHa2; simpl; reflexivity);
+    try (rewrite -> IHa2; simpl; reflexivity);
+    try (rewrite -> IHa1; simpl; rewrite plus_0_r; reflexivity).
+    + destruct n0; simpl in *.
+      * rewrite plus_0_r. auto.
+      * rewrite <- IHa1. rewrite <- IHa2. simpl. reflexivity.
+  - simpl.
+    rewrite <- IHa1. rewrite <- IHa2. reflexivity.
+  - simpl.
+    rewrite <- IHa1. rewrite <- IHa2. reflexivity.
 Qed.
 
 (*-- Check --*)
