sf/Assignment08_17.v
@@ -5,7 +5,17 @@ Require Export Assignment08_16.
 Lemma optimize_0plus_bexp_sound:
   btrans_sound optimize_0plus_bexp.
 Proof.
-  exact FILL_IN_HERE.
+  unfold btrans_sound. intros. unfold bequiv. intros.
+  induction b; try (simpl; reflexivity);
+  try (simpl;
+       repeat (rewrite <- optimize_0plus_aexp_sound);
+       reflexivity).
+  - simpl.
+    rewrite <- IHb.
+    reflexivity.
+  - simpl.
+    rewrite <- IHb1. rewrite <- IHb2.
+    reflexivity.
 Qed.
 
 (*-- Check --*)
