sf/Assignment08_18.v
@@ -5,7 +5,15 @@ Require Export Assignment08_17.
 Lemma optimize_0plus_com_sound:
   ctrans_sound optimize_0plus_com.
 Proof.
-  exact FILL_IN_HERE.
+  unfold ctrans_sound. intros.
+  induction c; simpl.
+  - apply refl_cequiv.
+  - apply CAss_congruence. apply optimize_0plus_aexp_sound.
+  - apply CSeq_congruence; auto.
+  - apply CIf_congruence; auto.
+    apply optimize_0plus_bexp_sound.
+  - apply CWhile_congruence; auto.
+    apply optimize_0plus_bexp_sound.
 Qed.
 
 (*-- Check --*)
